Imperia/Do/Elab.lean
@@ -1,4 +1,3 @@
-
 /-
 Copyright (c) 2024 Mac Malone. All rights reserved.
 Released under Apache 2.0 license as described in the file LICENSE.
@@ -6,9 +5,25 @@ Authors: Mac Malone
 -/
 import Imperia.Do.Basic
 
-open Lean Parser
+open Lean Elab Term.Do Parser
 
 namespace Imperia
+
+syntax (name := μdoScopes) "μdo_scopes%" : doElem
+
+@[μdo_elab μdoScopes]
+def elabMDoScopes : MDoElab := fun x xs expectedType? => do
+  let scopes ← getMDoScopes
+  let scopes := flip MessageData.joinSep "\n" <| scopes.stack.map fun scope =>
+    m!"· mutable vars: {scope.vars.toString}"
+  logInfoAt x m!"μdo scopes:{indentD scopes}"
+  elabMDoElems xs expectedType?
+
+@[μdo_elab μdoGoto]
+def elabMDoGoto : MDoElab := adaptMDoMacroElab fun x _ => do
+  let `(μdoGoto|μdo_goto% $x) := x
+    | throwErrorAt x "ill-formed `μdo_goto%` syntax"
+  applyMDoVars x
 
 @[μdo_elab μdoNested]
 def elabΜdoNested := adaptMDoMacro fun x xs => do
@@ -32,47 +47,81 @@ def elabDoExpr := adaptMDoMacro fun x xs => do
   mkMDoTerm x fun x => mkMDoAndThen x xs
 
 @[μdo_elab doLet]
-def elabDoLet := adaptMDoMacro fun x xs => do
-  let `(Term.doLet|let%$tk $[mut%$mutTk?]? $d:letDecl) := x
-    | Macro.throwErrorAt x "ill-formed `do` let syntax"
+def elabDoLet := adaptMDoMacroElab fun x xs => do
+  let `(Term.doLet|let%$tk $[mut%$mutTk?]? $decl:letDecl) := x
+    | throwErrorAt x "ill-formed `do` let syntax"
   withRef tk do
-  if let some tk := mutTk? then
-    Macro.throwErrorAt tk "`mut` has not been implemented for `μdo`"
+  declareMDoVars (← getLetDeclVars decl) mutTk?.isSome
   let body ← mkMDoOfElems xs
-  mkMDoTerm d fun d => `(let $d:letDecl; $body)
+  mkMDoTerm decl fun decl => `(let $decl:letDecl; $body)
 
 @[μdo_elab doLetElse]
-def elabDoLetElse := adaptMDoMacro fun x xs => do
+def elabDoLetElse := adaptMDoMacroElab fun x xs => do
   let `(Term.doLetElse|let%$tk $[mut%$mutTk?]? $pat := $v | $e:doSeq) := x
-    | Macro.throwErrorAt x "ill-formed `do` let syntax"
+    | throwErrorAt x "ill-formed `do` let syntax"
   withRef tk do
-  if let some tk := mutTk? then
-    Macro.throwErrorAt tk "`mut` has not been implemented for `μdo`"
+  declareMDoVars (← getPatternVarsEx pat) mutTk?.isSome
   let e ← mkMDoOfSeq e
   let body ← mkMDoOfElems xs
   mkMDoTerm v fun v => `(if let $pat := $v then $body else $e)
 
+@[inline]
+def mkMDoIdBind
+  [Monad m] [MonadQuotation m] (bindRef : Syntax)
+  (id : Ident) (ty? : Option Term) (v : DoElem) (xs : Array DoElem)
+: m Term := do
+  let body ← mkMDoOfElems xs
+  mkMDoBind bindRef (← mkMDoOfElem v) `(fun $id $[: $ty?]? => $body)
+
+@[inline]
+def mkMDoPatBind
+  [Monad m] [MonadQuotation m] (bindRef : Syntax)
+  (pat : Term) (v : DoElem) (e? : Option DoSeq) (xs : Array DoElem)
+: m Term := do
+  let patAlt ← `(Term.matchAltExpr| | $pat => $(← mkMDoOfElems xs))
+  let alts ← id do
+    if let some e := e? then
+      let eAlt ← withRef e `(Term.matchAltExpr| | _ => μdo% $(expandDoSeq e)*)
+      return #[patAlt, eAlt]
+    else
+      return #[patAlt]
+  mkMDoBind bindRef (← mkMDoOfElem v) `(fun $alts:matchAlt*)
+
 @[μdo_elab doLetArrow]
-def elabDoLetArrow := adaptMDoMacro fun x xs => do
+def elabDoLetArrow := adaptMDoMacroElab fun x xs => do
   let `(Term.doLetArrow|let%$letTk $[mut%$mutTk?]? $decl) := x
-    | Macro.throwErrorAt x "ill-formed `do` let syntax"
+    | throwErrorAt x "ill-formed `do` let syntax"
   withRef letTk do
-  if let some tk := mutTk? then
-    Macro.throwErrorAt tk "`mut` has not been implemented for `μdo`"
   match decl with
   | `(Term.doIdDecl|$id $[: $ty?]? ←%$bindTk $v) =>
-    let body ← mkMDoOfElems xs
-    mkMDoBind bindTk (← mkMDoOfElem v) `(fun $id $[: $ty?]? => $body)
+    declareMDoVar id mutTk?.isSome
+    mkMDoIdBind bindTk id ty? v xs
   | `(Term.doPatDecl|$pat ←%$bindTk $v $[| $e?]?) => do
-    let patAlt ← `(Term.matchAltExpr| | $pat => $(← mkMDoOfElems xs))
-    let alts ← id do
-      if let some e := e? then
-        let eAlt ← withRef e `(Term.matchAltExpr| | _ => μdo% $(← expandDoSeq e)*)
-        return #[patAlt, eAlt]
-      else
-        return #[patAlt]
-    mkMDoBind bindTk (← mkMDoOfElem v) `(fun $alts:matchAlt*)
-  | x => Macro.throwErrorAt x "ill-formed let declaration"
+    declareMDoVars (← getPatternVarsEx pat) mutTk?.isSome
+    mkMDoPatBind bindTk pat v e? xs
+  | x => throwErrorAt x "ill-formed let declaration"
+
+@[μdo_elab doReassign]
+def elabDoReassign := adaptMDoMacroElab fun x xs => withRef x do
+  match x with
+  | `(Term.doReassign|$id := $v) =>
+    checkMDoVarReassignable id.getId
+    `(let $id := $v; $(← mkMDoOfElems xs))
+  | `(Term.doReassign|$decl:letPatDecl) =>
+    checkMDoVarsReassignable (← getLetPatDeclVars decl)
+    `(let $decl:letPatDecl; $(← mkMDoOfElems xs))
+  | x => throwErrorAt x "ill-formed `do` reassignment syntax"
+
+@[μdo_elab doReassignArrow]
+def elabDoReassignArrow := adaptMDoMacroElab fun x xs => withRef x do
+  match x with
+  | `(Term.doReassignArrow|$id:ident $[: $ty?]? ←%$bindTk $v) =>
+    checkMDoVarReassignable id.getId
+    mkMDoIdBind bindTk id ty? v xs
+  | `(Term.doReassignArrow|$pat:term ←%$bindTk $v $[| $e?]?) =>
+    checkMDoVarsReassignable (← getPatternVarsEx pat)
+    mkMDoPatBind bindTk pat v e? xs
+  | x => throwErrorAt x "ill-formed `do` reassignment syntax"
 
 @[μdo_elab doMatch]
 def elabDoMatch := adaptMDoMacro fun x xs => do
@@ -106,10 +155,10 @@ def elabDoIf := adaptMDoMacro fun x xs => do
     | Macro.throwErrorAt x "ill-formed `do` if syntax"
   withRef tk do
   mkMDoJmp xs fun jmp => do
-  let e ← if let some e := e? then mkMDoSeqJmp e jmp else jmp.mkTerm
+  let e ← if let some e := e? then mkMDoBranch e jmp else jmp.mkTerm
   let e ← (ecs.zip ets).foldrM (init := e) fun (c, t) e => do
-    mkMDoIf c (← mkMDoSeqJmp t jmp) e
-  mkMDoIf c (← mkMDoSeqJmp t jmp) e
+    mkMDoIf c (← mkMDoBranch t jmp) e
+  mkMDoIf c (← mkMDoBranch t jmp) e
 
 @[μdo_elab doUnless]
 def elabDoUnless := adaptMDoMacro fun x xs => do
@@ -117,7 +166,7 @@ def elabDoUnless := adaptMDoMacro fun x xs => do
     | Macro.throwErrorAt x "ill-formed `do` unless syntax"
   withRef tk do
   mkMDoJmp xs fun jmp => do
-  let x ← mkMDoSeqJmp x jmp
+  let x ← mkMDoBranch x jmp
   let jmp ← jmp.mkTerm
   mkMDoTerm c fun c => `(if $c then $jmp else $x)
 
@@ -126,9 +175,8 @@ def elabDoReturn := adaptMDoMacro fun x xs => do
   let `(Term.doReturn|return%$tk $(v?)?) := x
     | Macro.throwErrorAt x "ill-formed `do` return syntax"
   withRef tk do
-  if xs.size > 0 then
-    Macro.throwErrorAt tk "return must be the last element in a `do` sequence"
-  else if let some v := v? then
+  checkTerminal "return" xs
+  if let some v := v? then
     mkMDoTerm v fun v => ``(ret $v)
   else
     ``(halt)
@@ -138,9 +186,8 @@ def elabDoRaise := adaptMDoMacro fun x xs => do
   let `(doRaise|raise%$tk $(v?)?) := x
     | Macro.throwErrorAt x "ill-formed `do` raise syntax"
   withRef tk do
-  if xs.size > 0 then
-    Macro.throwErrorAt tk "raise must be the last element in a `do` sequence"
-  else if let some v := v? then
+  checkTerminal "raise" xs
+  if let some v := v? then
     mkMDoTerm v fun v => ``(Throw.throw $v)
   else
     ``(Throw.throw ())
