Imperia/Util/Syntax.lean
@@ -5,6 +5,7 @@ Authors: Mac Malone
 -/
 import Lean.Parser
 import Imperia.Cont
+import Imperia.Util.MonadMacroError
 
 open Lean Parser Elab
 
@@ -29,8 +30,8 @@ def mkBinderIdentPat (x : TSyntax [identKind, ``Term.hole]) : Term := Unhygienic
 
 instance : Coe (TSyntax [identKind, ``Term.hole]) Term := ⟨mkBinderIdentPat⟩
 
-def expandDoSeq (x : DoSeq) : MacroM (Array DoElem) :=
+def expandDoSeq (x : DoSeq) : Array DoElem :=
   match x with
-  | `(Term.doSeq|$[$xs $[;]?]*) => pure xs
-  | `(Term.doSeq|{$[$xs $[;]?]*}) => pure xs
-  | x => Macro.throwErrorAt x "ill-formed `do` sequence"
+  | `(Term.doSeq|$[$xs $[;]?]*) => xs
+  | `(Term.doSeq|{$[$xs $[;]?]*}) => xs
+  | _ => #[]
